src/HigherValue.v
@@ -1,4 +1,5 @@
 Require Import Common.
+Require Import Metadata.
 
 Definition function_name := nat.
 
@@ -64,3 +65,14 @@ Definition value_ind' (P : value -> Prop)
     (v : value) : P v :=
     ltac:(refine (@value_rect_mut P (Forall P)
         HConstr HClose _ _ v); eauto).
+
+
+Inductive public_value (M : list metadata) : value -> Prop :=
+| PvConstr : forall tag args,
+        Forall (public_value M) args ->
+        public_value M (Constr tag args)
+| PvClose : forall fname free,
+        public_fname M fname ->
+        Forall (public_value M) free ->
+        public_value M (Close fname free).
+
