src/ElimFunc.v
@@ -404,12 +404,15 @@ Inductive is_callstate (prog : prog_type) : valtype -> valtype -> state -> Prop 
         let fv := HigherValue.Close fname free in
         expr_value ae av ->
         Forall2 expr_value free_e free ->
+        HigherValue.public_value (snd prog) fv ->
+        HigherValue.public_value (snd prog) av ->
         is_callstate prog fv av
             (Run body (ae :: free_e) Stop).
 
 Inductive final_state (prog : prog_type) : state -> valtype -> Prop :=
 | FinalState : forall e v,
         expr_value e v ->
+        HigherValue.public_value (snd prog) v ->
         final_state prog (Stop e) v.
 
 Definition initial_env (prog : prog_type) : env := fst prog.
